Basic pred work

rocq-bluerock-brick/theories/lang/cpp/model/inductive_pred2.v
@@ -1,3 +1,15 @@
+Require Import iris.algebra.excl.
+Require Import iris.algebra.gmap.
+Require Import iris.algebra.lib.frac_auth.
+Require Import iris.bi.monpred.
+Require Import iris.bi.lib.fractional.
+Require Import bedrock.lang.proofmode.proofmode.
+
+Require Import bedrock.lang.bi.fractional.
+Require Import bedrock.lang.bi.cancelable_invariants.
+Require Import bedrock.lang.cpp.bi.cfractional.
+Require Import bedrock.lang.base_logic.own_instances.
+
 Require Import bedrock.lang.cpp.logic.mpred.
 Require Import bedrock.lang.cpp.logic.pred2.
 Require Import bedrock.lang.cpp.semantics.values2.
@@ -7,8 +19,202 @@ Require Import bedrock.lang.cpp.model.inductive_pointers2.
 Ensures that everything needed is properly functorized. *)
 Import PTRS_IMPL.
 
+(* todo: does this not exist as a library somewhere? *)
+Definition cfractionalR (V : Type) : cmra :=
+  prodR cQp.tR (agreeR (leibnizO V)).
+Definition cfrac {V : Type} q (v : V) : cfractionalR V :=
+  (q, to_agree v).
+
+Lemma cfrac_op {V} (l : V) q1 q2 :
+  cfrac q1 l ⋅ cfrac q2 l ≡ cfrac (q1 ⋅ q2) l.
+Proof. by rewrite -pair_op agree_idemp. Qed.
+
+Lemma cfrac_valid {A : Type} {q1 q2} {v1 v2 : A} :
+  ✓ (cfrac q1 v1 ⋅ cfrac q2 v2) → ✓ (q1 ⋅ q2)%Qp ∧ v1 = v2.
+Proof. by move /pair_valid => /= []? /to_agree_op_inv_L. Qed.
+
+Section fractional.
+  Context {K V : Type} `{Countable K} `{!HasOwn PROP (gmapR K (cfractionalR V))}.
+
+  Let gmap_own γ q k v :=
+    own (A := gmapR K (cfractionalR V)) γ {[ k := cfrac q v ]}.
+  #[global] Instance cfractional_own_frac γ k v :
+    CFractional (λ q, gmap_own γ q k v).
+  Proof. intros q1 q2. by rewrite -own_op singleton_op cfrac_op. Qed.
+
+  #[global] Instance fractional_own_frac_as_fractional γ k v q :
+    AsCFractional (gmap_own γ q k v) (λ q, gmap_own γ q k v) q.
+  Proof. solve_as_cfrac. Qed.
+
+  #[global] Instance gmap_own_agree
+    `{!BiEmbed siPropI PROP} `{!HasOwnValid PROP (gmapR K (cfractionalR V))}
+    v1 v2 γ q1 q2 k :
+    Observe2 [| v1 = v2 |] (gmap_own γ q1 k v1) (gmap_own γ q2 k v2).
+  Proof.
+    apply: observe_2_intro_only_provable.
+    apply bi.wand_intro_r; rewrite /gmap_own -own_op singleton_op.
+    rewrite own_valid discrete_valid singleton_valid.
+    by iIntros "!%" => /cfrac_valid [].
+  Qed.
+
+  (**
+  We keep this instance local because guarding it with [CFracValid2]
+  prevents it from firing. (Perhaps due to the let binding.)
+  *)
+  Instance gmap_own_cfrac_valid γ
+    `{!BiEmbed siPropI PROP} `{!HasOwnValid PROP (gmapR K (cfractionalR V))} :
+    ∀ q k v, Observe [| cQp.frac q ≤ 1 |]%Qp (gmap_own γ q k v).
+  Proof.
+    intros. apply: observe_intro_only_provable.
+    rewrite /gmap_own own_valid !discrete_valid singleton_valid.
+    by iIntros "!%" => /pair_valid [? _].
+  Qed.
+End fractional.
+#[local] Existing Instance gmap_own_cfrac_valid.
+
 Declare Module Import VALUES_DEFS_IMPL : VALUES_INTF_FUNCTOR PTRS_IMPL.
 
+Existing Instance ptr_countable.
+
+#[local] Set Printing Coercions.
+
+Implicit Types (vt : validity_type) (σ : genv) (q : cQp.t).
+
 Module CPP_BASE <: CPP_LOGIC_CLASS.
+  Definition addr : Set := N.
+  Definition byte : Set := N.
+  
+  Record cpp_ghost' : Type := {
+    blocks_name : gname
+  }.
+  Definition _cpp_ghost := cpp_ghost'.
+
+  Record cppG' (Σ : gFunctors) : Type := {
+    (* Maps pointers to each block's start and size *)
+    blocksG : inG Σ (gmapUR ptr (agreeR (leibnizO (N * N))));
+    has_inv' : invGS Σ;
+    has_cinv' : cinvG Σ
+  }.
+
+  Definition cppPreG := cppG'.
+
+  Definition has_inv Σ : cppPreG Σ -> invGS Σ := @has_inv' Σ.
+  Definition has_cinv Σ : cppPreG Σ -> cinvG Σ := @has_cinv' Σ.
+  
+  Include CPP_LOGIC_CLASS_MIXIN.
+
+  Section with_cpp.
+    Context `{!cpp_logic thread_info Σ}.
+
+    Existing Class cppG'.
+    #[local] Instance cppPreG_cppG' : cppG' Σ := cpp_has_cppG.
+    #[local] Existing Instances blocksG.
+
+    Definition blocks_own (p : ptr) (s e : N) : mpred :=
+      own (A := gmapUR ptr (agreeR (leibnizO (N * N))))
+        cpp_ghost.(blocks_name) {[ p := to_agree (s, e) ]}.
+  End with_cpp.
 
 End CPP_BASE.
+
+(* Module Type CPP_VIRTUAL.
+  Import CPP_BASE.
+
+  Parameter vbyte : forall `{!cpp_logic thread_info Σ}
+    (va : addr) (rv : runtime_val') (q : Qp), mpred.
+  Section with_cpp.
+    Context `{cpp_logic}.
+
+    Axiom vbyte_fractional : forall va rv, Fractional (vbyte va rv).
+    Axiom vbyte_timeless : forall va rv q, Timeless (vbyte va rv q).
+    #[global] Existing Instances vbyte_fractional vbyte_timeless.
+
+    Definition vbytes (a : addr) (rv : list runtime_val') (q : Qp) : mpred :=
+      [∗list] o ↦ v ∈ rv, (vbyte (a+N.of_nat o)%N v q).
+
+    #[global] Instance vbytes_fractional va rv : Fractional (vbytes va rv).
+    Proof. apply fractional_big_sepL; intros. apply vbyte_fractional. Qed.
+
+    #[global] Instance vbytes_as_fractional va rv q :
+      AsFractional (vbytes va rv q) (vbytes va rv) q.
+    Proof. exact: Build_AsFractional. Qed.
+
+    #[global] Instance vbytes_timeless va rv q : Timeless (vbytes va rv q) := _.
+  End with_cpp.
+End CPP_VIRTUAL. *)
+
+Module CPP <: CPP_LOGIC.
+  Import CPP_BASE.
+
+  Section with_cpp.
+    Context `{cpp_logic}.
+
+    Definition _valid_ptr `{σ : genv} vt (p : ptr) : mpred :=
+      match vt with
+      | Relaxed =>
+        [| p = nullptr |] \\//
+        Exists base s e,
+          blocks_own base s e **
+          [|
+            ∃ o no,
+              (s <= no <= s + e)%N /\
+              ptr_vaddr σ p <> Some 0%N /\
+              eval_offset σ o = Some (Z.of_N no) /\
+              p = base ,, o
+          |]
+      | Strict =>
+        Exists base s e,
+          blocks_own base s e **
+          [|
+            ∃ o no,
+              (s <= no < s + e)%N /\
+              ptr_vaddr σ p <> Some 0%N /\
+              eval_offset σ o = Some (Z.of_N no) /\
+              p = base ,, o
+          |]
+      end.
+    
+    Notation strict_valid_ptr := (_valid_ptr Strict).
+    (* relaxed validity (past-the-end allowed) *)
+    Notation valid_ptr := (_valid_ptr Relaxed).
+
+    Instance _valid_ptr_persistent `{genv} : ∀ b p, Persistent (_valid_ptr b p).
+    Admitted.
+    Instance _valid_ptr_affine `{genv} : ∀ b p, Affine (_valid_ptr b p).
+    Admitted.
+    Instance _valid_ptr_timeless `{genv} : ∀ b p, Timeless (_valid_ptr b p).
+    Admitted.
+
+    Lemma valid_ptr_nullptr `{genv} :
+      |-- valid_ptr nullptr.
+    Proof. now iLeft. Qed.
+
+    Lemma not_strictly_valid_ptr_nullptr `{genv} :
+      strict_valid_ptr nullptr |-- False.
+    Proof.
+      iIntros "H". rewrite /strict_valid_ptr.
+      iDestruct "H" as (???) "[H1 H2]".
+      iDestruct "H2" as (??) "H2".
+      iDestruct "H2" as "(%H2 & %H3)".
+      simpl in *. now destruct H3.
+    Qed.
+      
+    Lemma strict_valid_valid `{genv} :
+      ∀ p,
+        strict_valid_ptr p |-- valid_ptr p.
+    Proof.
+      intros.
+      rewrite /strict_valid_ptr /valid_ptr.
+      iIntros "H". iRight.
+      iDestruct "H" as (base s e) "H".
+      iExists base, s, e.
+      iDestruct "H" as "[H1 H2]".
+      iSplit. iAssumption.
+      iDestruct "H2" as (o no) "H2".
+      iDestruct "H2" as "[%H2 H3]".
+      iExists o, no. iSplit.
+      { iPureIntro. lia. }
+      { iAssumption. }
+    Qed.
+
+End CPP.
