rocq-bluerock-brick/theories/lang/cpp/semantics/ptrs2.v
@@ -304,6 +304,7 @@ Module Type PTRS.
   (** [eval_offset] and associated axioms are more advanced, only to be used
   in special cases. *)
   (* TODO drop [genv]. *)
+  (* TODO change Z to N *)
   Parameter eval_offset : genv -> offset -> option Z.
 
   Axiom eval_o_sub : forall σ ty (i : Z),
